Strata/DL/Lambda/IntBoolFactory.lean
@@ -46,20 +46,20 @@ def binaryPredicate (n : T.Identifier)
     concreteEval := ceval }
 
 def unOpCeval (InTy OutTy : Type) [ToString OutTy]
-                (cevalInTy : (LExpr T.mono) → Option InTy) (op : InTy → OutTy)
-                (ty : LMonoTy) :
+                (mkConst : T.Metadata → OutTy → LExpr T.mono)
+                (cevalInTy : (LExpr T.mono) → Option InTy) (op : InTy → OutTy) :
                 (LExpr T.mono) → List (LExpr T.mono) → (LExpr T.mono) :=
   (fun e args => match args with
    | [e1] =>
      let e1i := cevalInTy e1
      match e1i with
-     | some x => (LExpr.const e1.metadata (toString (op x)) ty)
+     | some x => mkConst e1.metadata (op x)
      | _ => e
    | _ => e)
 
 def binOpCeval (InTy OutTy : Type) [ToString OutTy]
-                (cevalInTy : (LExpr T.mono) → Option InTy) (op : InTy → InTy → OutTy)
-                (ty : LMonoTy) :
+                (mkConst : T.Metadata → OutTy → LExpr T.mono)
+                (cevalInTy : LExpr T.mono → Option InTy) (op : InTy → InTy → OutTy) :
                 (LExpr T.mono) → List (LExpr T.mono) → (LExpr T.mono) :=
   (fun e args => match args with
    | [e1, e2] =>
@@ -100,15 +100,15 @@ def cevalIntMod (e : LExpr T.mono) (args : List (LExpr T.mono)) : LExpr T.mono :
 
 def intAddFunc : LFunc T :=
   binaryOp "Int.Add" .int
-  (some (binOpCeval Int Int intConst LExpr.denoteInt Int.add))
+  (some (binOpCeval Int Int (@intConst T.mono) LExpr.denoteInt Int.add))
 
 def intSubFunc : LFunc T :=
   binaryOp "Int.Sub" .int
-  (some (binOpCeval Int Int intConst LExpr.denoteInt Int.sub))
+  (some (binOpCeval Int Int (@intConst T.mono) LExpr.denoteInt Int.sub))
 
 def intMulFunc : LFunc T :=
   binaryOp "Int.Mul" .int
-  (some (binOpCeval Int Int intConst LExpr.denoteInt Int.mul))
+  (some (binOpCeval Int Int (@intConst T.mono) LExpr.denoteInt Int.mul))
 
 def intDivFunc : LFunc T :=
   binaryOp "Int.Div" .int
@@ -120,44 +120,44 @@ def intModFunc : LFunc T :=
 
 def intNegFunc : LFunc T :=
   unaryOp "Int.Neg" .int
-  (some (unOpCeval Int Int intConst LExpr.denoteInt Int.neg))
+  (some (unOpCeval Int Int (@intConst T.mono) LExpr.denoteInt Int.neg))
 
 def intLtFunc : LFunc T :=
   binaryPredicate "Int.Lt" .int
-  (some (binOpCeval Int Bool boolConst LExpr.denoteInt (fun x y => x < y)))
+  (some (binOpCeval Int Bool (@boolConst T.mono) LExpr.denoteInt (fun x y => x < y)))
 
 def intLeFunc : LFunc T :=
   binaryPredicate "Int.Le" .int
-  (some (binOpCeval Int Bool boolConst LExpr.denoteInt (fun x y => x <= y)))
+  (some (binOpCeval Int Bool (@boolConst T.mono) LExpr.denoteInt (fun x y => x <= y)))
 
 def intGtFunc : LFunc T :=
   binaryPredicate "Int.Gt" .int
-  (some (binOpCeval Int Bool boolConst LExpr.denoteInt (fun x y => x > y)))
+  (some (binOpCeval Int Bool (@boolConst T.mono) LExpr.denoteInt (fun x y => x > y)))
 
 def intGeFunc : LFunc T :=
   binaryPredicate "Int.Ge" .int
-  (some (binOpCeval Int Bool boolConst LExpr.denoteInt (fun x y => x >= y)))
+  (some (binOpCeval Int Bool (@boolConst T.mono) LExpr.denoteInt (fun x y => x >= y)))
 
 /- Boolean Operations -/
 def boolAndFunc : LFunc T :=
   binaryOp "Bool.And" .bool
-  (some (binOpCeval Bool Bool boolConst LExpr.denoteBool Bool.and))
+  (some (binOpCeval Bool Bool (@boolConst T.mono) LExpr.denoteBool Bool.and))
 
 def boolOrFunc : LFunc T :=
   binaryOp "Bool.Or" .bool
-  (some (binOpCeval Bool Bool boolConst LExpr.denoteBool Bool.or))
+  (some (binOpCeval Bool Bool (@boolConst T.mono) LExpr.denoteBool Bool.or))
 
 def boolImpliesFunc : LFunc T :=
   binaryOp "Bool.Implies" .bool
-  (some (binOpCeval Bool Bool boolConst LExpr.denoteBool (fun x y => ((not x) || y))))
+  (some (binOpCeval Bool Bool (@boolConst T.mono) LExpr.denoteBool (fun x y => ((not x) || y))))
 
 def boolEquivFunc : LFunc T :=
   binaryOp "Bool.Equiv" .bool
-  (some (binOpCeval Bool Bool boolConst LExpr.denoteBool (fun x y => (x == y))))
+  (some (binOpCeval Bool Bool (@boolConst T.mono) LExpr.denoteBool (fun x y => (x == y))))
 
 def boolNotFunc : LFunc T :=
   unaryOp "Bool.Not" .bool
-  (some (unOpCeval Bool Bool boolConst LExpr.denoteBool Bool.not))
+  (some (unOpCeval Bool Bool (@boolConst T.mono) LExpr.denoteBool Bool.not))
 
 def IntBoolFactory : @Factory T :=
   open LTy.Syntax in #[
