Strata/DL/Lambda/LExpr.lean
@@ -65,6 +65,9 @@ Dot notation syntax: T.mono transforms LExprParams into LExprParamsT with LMonoT
 abbrev LExprParams.mono (T : LExprParams) : LExprParamsT :=
   ⟨T, LMonoTy⟩
 
+abbrev identifier := Identifier
+abbrev LExprParams.Identifier (T : LExprParams) := identifier T.IDMeta
+
 structure Typed (T: Type) where
   underlying: T
   type: LMonoTy
@@ -651,7 +654,9 @@ Syntax for conveniently building `LExpr` terms with `LMonoTy`, scoped under the 
 namespace SyntaxMono
 open Lean Elab Meta
 
-class MkLExprParams (T : LExprParams) where
+-- Although T is not used in the class, it makes it possible to create instances
+-- so that toExpr is meant to be typed
+class MkLExprParams (T: LExprParams) where
   elabIdent : Lean.Syntax → MetaM Expr
   toExpr : Expr
 
@@ -678,7 +683,7 @@ scoped syntax lconstmono : lexprmono
 def mkIntLit (n: NumLit) : Expr := Expr.app (.const ``Int.ofNat []) (mkNatLit n.getNat)
 def mkNegLit (n: NumLit) := Expr.app (.const ``Int.neg []) (mkIntLit n)
 
-def elabLConstMono (T: LExprParams) [MkLExprParams T] : Lean.Syntax → MetaM Expr
+def elabLConstMono [MkLExprParams T] : Lean.Syntax → MetaM Expr
   | `(lconstmono| #$n:num)  => do
     let metadata ← mkAppM ``Unit.unit #[]
     let tMono ← mkAppM ``LExprParams.mono #[MkLExprParams.toExpr T]
@@ -714,7 +719,7 @@ scoped syntax "~" noWs lidentmono : lopmono
 scoped syntax "(" lopmono ":" lmonoty ")" : lopmono
 scoped syntax lopmono : lexprmono
 
-def elabLOpMono (T : LExprParams)  [MkLExprParams T] : Lean.Syntax → MetaM Expr
+def elabLOpMono [MkLExprParams T] : Lean.Syntax → MetaM Expr
   | `(lopmono| ~$s:lidentmono)  => do
     let none ← mkNone (mkConst ``LMonoTy)
     let metadata ← mkAppM ``Unit.unit #[]
@@ -730,7 +735,7 @@ def elabLOpMono (T : LExprParams)  [MkLExprParams T] : Lean.Syntax → MetaM Exp
 
 declare_syntax_cat lbvarmono
 scoped syntax "%" noWs num : lbvarmono
-def elabLBVarMono (T : LExprParams)  [MkLExprParams T] : Lean.Syntax → MetaM Expr
+def elabLBVarMono [MkLExprParams T] : Lean.Syntax → MetaM Expr
   | `(lbvarmono| %$n:num) => do
     let metadata ← mkAppM ``Unit.unit #[]
     let tMono ← mkAppM ``LExprParams.mono #[MkLExprParams.toExpr T]
@@ -742,7 +747,7 @@ declare_syntax_cat lfvarmono
 scoped syntax lidentmono : lfvarmono
 scoped syntax "(" lidentmono ":" lmonoty ")" : lfvarmono
 
-def elabLFVarMono (T : LExprParams)  [MkLExprParams T] : Lean.Syntax → MetaM Expr
+def elabLFVarMono [MkLExprParams T] : Lean.Syntax → MetaM Expr
   | `(lfvarmono| $i:lidentmono) => do
     let none ← mkNone (mkConst ``LMonoTy)
     let metadata ← mkAppM ``Unit.unit #[]
@@ -794,95 +799,95 @@ All type annotations in `LExpr` are for monotypes, not polytypes. It's the
 user's responsibility to ensure correct usage of type variables (i.e., they're
 unique).
 -/
-partial def elabLExprMono (T : LExprParams) [MkLExprParams T] : Lean.Syntax → MetaM Expr
-  | `(lexprmono| $c:lconstmono) => elabLConstMono T c
-  | `(lexprmono| $o:lopmono) => elabLOpMono T o
-  | `(lexprmono| $b:lbvarmono) => elabLBVarMono T b
-  | `(lexprmono| $f:lfvarmono) => elabLFVarMono T f
+partial def elabLExprMono [MkLExprParams T] : Lean.Syntax → MetaM Expr
+  | `(lexprmono| $c:lconstmono) => elabLConstMono (T:=T) c
+  | `(lexprmono| $o:lopmono) => elabLOpMono (T:=T) o
+  | `(lexprmono| $b:lbvarmono) => elabLBVarMono (T:=T) b
+  | `(lexprmono| $f:lfvarmono) => elabLFVarMono (T:=T) f
   | `(lexprmono| λ $e:lexprmono) => do
-     let e' ← elabLExprMono T e
+     let e' ← elabLExprMono (T:=T) e
      let tMono ← mkAppM ``LExprParams.mono #[MkLExprParams.toExpr T]
      let metadata ← mkAppM ``Unit.unit #[]
      return mkAppN (.const ``LExpr.absUntyped []) #[tMono, metadata, e']
   | `(lexprmono| λ ($mty:lmonoty): $e:lexprmono) => do
      let lmonoty ← Lambda.LTy.Syntax.elabLMonoTy mty
      let lmonoty ← mkSome (mkConst ``LMonoTy) lmonoty
-     let e' ← elabLExprMono T e
+     let e' ← elabLExprMono (T:=T) e
      let tMono ← mkAppM ``LExprParams.mono #[MkLExprParams.toExpr T]
      let metadata ← mkAppM ``Unit.unit #[]
      return mkAppN (.const ``LExpr.abs []) #[tMono, metadata, lmonoty, e']
   | `(lexprmono| ∀ $e:lexprmono) => do
-     let e' ← elabLExprMono T e
+     let e' ← elabLExprMono (T:=T) e
      let tMono ← mkAppM ``LExprParams.mono #[MkLExprParams.toExpr T]
      let metadata ← mkAppM ``Unit.unit #[]
      return mkAppN (.const ``LExpr.allUntyped []) #[tMono, metadata, e']
   | `(lexprmono| ∀ {$tr}$e:lexprmono) => do
-     let e' ← elabLExprMono T e
-     let tr' ← elabLExprMono T tr
+     let e' ← elabLExprMono (T:=T) e
+     let tr' ← elabLExprMono (T:=T) tr
      let tMono ← mkAppM ``LExprParams.mono #[MkLExprParams.toExpr T]
      let metadata ← mkAppM ``Unit.unit #[]
      return mkAppN (.const ``LExpr.allUntypedTr []) #[tMono, metadata, tr', e']
   | `(lexprmono| ∀ ($mty:lmonoty): $e:lexprmono) => do
      let lmonoty ← Lambda.LTy.Syntax.elabLMonoTy mty
      let lmonoty ← mkSome (mkConst ``LMonoTy) lmonoty
-     let e' ← elabLExprMono T e
+     let e' ← elabLExprMono (T:=T) e
      let tMono ← mkAppM ``LExprParams.mono #[MkLExprParams.toExpr T]
      let metadata ← mkAppM ``Unit.unit #[]
      return mkAppN (.const ``LExpr.all []) #[tMono, metadata, lmonoty, e']
   | `(lexprmono| ∀ ($mty:lmonoty):{$tr} $e:lexprmono) => do
      let lmonoty ← Lambda.LTy.Syntax.elabLMonoTy mty
      let lmonoty ← mkSome (mkConst ``LMonoTy) lmonoty
-     let e' ← elabLExprMono T e
-     let tr' ← elabLExprMono T tr
+     let e' ← elabLExprMono (T:=T) e
+     let tr' ← elabLExprMono (T:=T) tr
      let tMono ← mkAppM ``LExprParams.mono #[MkLExprParams.toExpr T]
      let metadata ← mkAppM ``Unit.unit #[]
      return mkAppN (.const ``LExpr.allTr []) #[tMono, metadata, lmonoty, tr', e']
   | `(lexprmono| ∃ ($mty:lmonoty): $e:lexprmono) => do
      let lmonoty ← Lambda.LTy.Syntax.elabLMonoTy mty
      let lmonoty ← mkSome (mkConst ``LMonoTy) lmonoty
-     let e' ← elabLExprMono T e
+     let e' ← elabLExprMono (T:=T) e
      let tMono ← mkAppM ``LExprParams.mono #[MkLExprParams.toExpr T]
      let metadata ← mkAppM ``Unit.unit #[]
      return mkAppN (.const ``LExpr.exist []) #[tMono, metadata, lmonoty, e']
   | `(lexprmono| ∃ ($mty:lmonoty):{$tr} $e:lexprmono) => do
      let lmonoty ← Lambda.LTy.Syntax.elabLMonoTy mty
      let lmonoty ← mkSome (mkConst ``LMonoTy) lmonoty
-     let e' ← elabLExprMono T e
-     let tr' ← elabLExprMono T tr
+     let e' ← elabLExprMono (T:=T) e
+     let tr' ← elabLExprMono (T:=T) tr
      let tMono ← mkAppM ``LExprParams.mono #[MkLExprParams.toExpr T]
      let metadata ← mkAppM ``Unit.unit #[]
      return mkAppN (.const ``LExpr.existTr []) #[tMono, metadata, lmonoty, tr', e']
   | `(lexprmono| ∃ $e:lexprmono) => do
-     let e' ← elabLExprMono T e
+     let e' ← elabLExprMono (T:=T) e
      let metadata ← mkAppM ``Unit.unit #[]
      let tMono ← mkAppM ``LExprParams.mono #[MkLExprParams.toExpr T]
      return mkAppN (.const ``LExpr.existUntyped []) #[tMono, metadata, e']
   | `(lexprmono| ∃{$tr} $e:lexprmono) => do
-     let e' ← elabLExprMono T e
-     let tr' ← elabLExprMono T tr
+     let e' ← elabLExprMono (T:=T) e
+     let tr' ← elabLExprMono (T:=T) tr
      let metadata ← mkAppM ``Unit.unit #[]
      let tMono ← mkAppM ``LExprParams.mono #[MkLExprParams.toExpr T]
      return mkAppN (.const ``LExpr.existUntypedTr []) #[tMono, metadata, tr', e']
   | `(lexprmono| ($e1:lexprmono $e2:lexprmono)) => do
-     let e1' ← elabLExprMono T e1
-     let e2' ← elabLExprMono T e2
+     let e1' ← elabLExprMono (T:=T) e1
+     let e2' ← elabLExprMono (T:=T) e2
      let metadata ← mkAppM ``Unit.unit #[]
      let tMono ← mkAppM ``LExprParams.mono #[MkLExprParams.toExpr T]
      return mkAppN (.const ``LExpr.app []) #[tMono, metadata, e1', e2']
   | `(lexprmono| $e1:lexprmono == $e2:lexprmono) => do
-     let e1' ← elabLExprMono T e1
-     let e2' ← elabLExprMono T e2
+     let e1' ← elabLExprMono (T:=T) e1
+     let e2' ← elabLExprMono (T:=T) e2
      let metadata ← mkAppM ``Unit.unit #[]
      let tMono ← mkAppM ``LExprParams.mono #[MkLExprParams.toExpr T]
      return mkAppN (.const ``LExpr.eq []) #[tMono, metadata, e1', e2']
   | `(lexprmono| if $e1:lexprmono then $e2:lexprmono else $e3:lexprmono) => do
-     let e1' ← elabLExprMono T e1
-     let e2' ← elabLExprMono T e2
-     let e3' ← elabLExprMono T e3
+     let e1' ← elabLExprMono (T:=T) e1
+     let e2' ← elabLExprMono (T:=T) e2
+     let e3' ← elabLExprMono (T:=T) e3
      let metadata ← mkAppM ``Unit.unit #[]
      let tMono ← mkAppM ``LExprParams.mono #[MkLExprParams.toExpr T]
      return mkAppN (.const ``LExpr.ite []) #[tMono, metadata, e1', e2', e3']
-  | `(lexprmono| ($e:lexprmono)) => elabLExprMono T e
+  | `(lexprmono| ($e:lexprmono)) => elabLExprMono (T:=T) e
   | _ => throwUnsupportedSyntax
 
 scoped syntax ident : lidentmono
@@ -997,7 +1002,9 @@ Syntax for conveniently building `LExpr` terms with `LTy`, scoped under the name
 namespace Syntax
 open Lean Elab Meta
 
-class MkLExprParams (IDMeta : Type) where
+-- Although T is not used in the class, it makes it possible to create instances
+-- so that toExpr is meant to be typed
+class MkLExprParams (T: LExprParams) where
   elabIdent : Lean.Syntax → MetaM Expr
   toExpr : Expr
 
@@ -1024,33 +1031,33 @@ scoped syntax lconst : lexpr
 def mkIntLit (n: NumLit) : Expr := Expr.app (.const ``Int.ofNat []) (mkNatLit n.getNat)
 def mkNegLit (n: NumLit) := Expr.app (.const ``Int.neg []) (mkIntLit n)
 
-def elabLConst (IDMeta : Type) [MkLExprParams IDMeta] : Lean.Syntax → MetaM Expr
+def elabLConst [MkLExprParams T] : Lean.Syntax → MetaM Expr
   | `(lconst| #$n:num)  => do
     let metadata ← mkAppM ``Unit.unit #[]
-    let baseParams := mkApp2 (mkConst ``LExprParams.mk) (mkConst ``Unit) (MkLExprParams.toExpr IDMeta)
+    let baseParams := MkLExprParams.toExpr T
     let tParams := mkApp2 (mkConst ``LExprParamsT.mk) baseParams (mkConst ``LTy)
     let lconstVal ← mkAppM ``LConst.intConst #[mkIntLit n]
     return mkAppN (.const ``LExpr.const []) #[tParams, metadata, lconstVal]
   | `(lconst| #-$n:num) => do
     let metadata ← mkAppM ``Unit.unit #[]
-    let baseParams := mkApp2 (mkConst ``LExprParams.mk) (mkConst ``Unit) (MkLExprParams.toExpr IDMeta)
+    let baseParams := MkLExprParams.toExpr T
     let tParams := mkApp2 (mkConst ``LExprParamsT.mk) baseParams (mkConst ``LTy)
     let lconstVal ← mkAppM ``LConst.intConst #[mkNegLit n]
     return mkAppN (.const ``LExpr.const []) #[tParams, metadata, lconstVal]
   | `(lconst| #true)    => do
     let metadata ← mkAppM ``Unit.unit #[]
-    let baseParams := mkApp2 (mkConst ``LExprParams.mk) (mkConst ``Unit) (MkLExprParams.toExpr IDMeta)
+    let baseParams := MkLExprParams.toExpr T
     let tParams := mkApp2 (mkConst ``LExprParamsT.mk) baseParams (mkConst ``LTy)
     return mkAppN (.const ``LExpr.boolConst []) #[tParams, metadata, toExpr true]
   | `(lconst| #false)   =>  do
     let metadata ← mkAppM ``Unit.unit #[]
-    let baseParams := mkApp2 (mkConst ``LExprParams.mk) (mkConst ``Unit) (MkLExprParams.toExpr IDMeta)
+    let baseParams := MkLExprParams.toExpr T
     let tParams := mkApp2 (mkConst ``LExprParamsT.mk) baseParams (mkConst ``LTy)
     return mkAppN (.const ``LExpr.boolConst []) #[tParams, metadata, toExpr false]
   | `(lconst| #$s:ident) => do
     let s := toString s.getId
     let metadata ← mkAppM ``Unit.unit #[]
-    let baseParams := mkApp2 (mkConst ``LExprParams.mk) (mkConst ``Unit) (MkLExprParams.toExpr IDMeta)
+    let baseParams := MkLExprParams.toExpr T
     let tParams := mkApp2 (mkConst ``LExprParamsT.mk) baseParams (mkConst ``LTy)
     return mkAppN (.const ``LExpr.const []) #[tParams, metadata, mkStrLit s]
   | _ => throwUnsupportedSyntax
@@ -1060,30 +1067,30 @@ scoped syntax "~" noWs lident : lop
 scoped syntax "(" lop ":" lty ")" : lop
 scoped syntax lop : lexpr
 
-def elabLOp (IDMeta : Type) [MkLExprParams IDMeta] : Lean.Syntax → MetaM Expr
+def elabLOp [MkLExprParams T] : Lean.Syntax → MetaM Expr
   | `(lop| ~$s:lident)  => do
     let none ← mkNone (mkConst ``LTy)
-    let ident ← MkLExprParams.elabIdent IDMeta s
+    let ident ← MkLExprParams.elabIdent T s
     let metadata ← mkAppM ``Unit.unit #[]
-    let baseParams := mkApp2 (mkConst ``LExprParams.mk) (mkConst ``Unit) (MkLExprParams.toExpr IDMeta)
+    let baseParams := MkLExprParams.toExpr T
     let tParams := mkApp2 (mkConst ``LExprParamsT.mk) baseParams (mkConst ``LTy)
     return mkAppN (.const ``LExpr.op []) #[tParams, metadata, ident, none]
   | `(lop| (~$s:lident : $ty:lty)) => do
     let lty ← Lambda.LTy.Syntax.elabLTy ty
     let lty ← mkSome (mkConst ``LTy) lty
     let metadata ← mkAppM ``Unit.unit #[]
-    let baseParams := mkApp2 (mkConst ``LExprParams.mk) (mkConst ``Unit) (MkLExprParams.toExpr IDMeta)
+    let baseParams := MkLExprParams.toExpr T
     let tParams := mkApp2 (mkConst ``LExprParamsT.mk) baseParams (mkConst ``LTy)
-    return mkAppN (.const ``LExpr.op []) #[tParams, metadata, ← MkLExprParams.elabIdent IDMeta s, lty]
+    return mkAppN (.const ``LExpr.op []) #[tParams, metadata, ← MkLExprParams.elabIdent T s, lty]
   | _ => throwUnsupportedSyntax
 
 declare_syntax_cat lbvar
 scoped syntax "%" noWs num : lbvar
 
-def elabLBVar (IDMeta : Type) [MkLExprParams IDMeta] : Lean.Syntax → MetaM Expr
+def elabLBVar [MkLExprParams T] : Lean.Syntax → MetaM Expr
   | `(lbvar| %$n:num) => do
     let metadata ← mkAppM ``Unit.unit #[]
-    let baseParams := mkApp2 (mkConst ``LExprParams.mk) (mkConst ``Unit) (MkLExprParams.toExpr IDMeta)
+    let baseParams := MkLExprParams.toExpr T
     let tParams := mkApp2 (mkConst ``LExprParamsT.mk) baseParams (mkConst ``LTy)
     return mkAppN (.const ``LExpr.bvar []) #[tParams, metadata, mkNatLit n.getNat]
   | _ => throwUnsupportedSyntax
@@ -1093,20 +1100,20 @@ declare_syntax_cat lfvar
 scoped syntax lident : lfvar
 scoped syntax "(" lident ":" lty ")" : lfvar
 
-def elabLFVar (IDMeta : Type) [MkLExprParams IDMeta] : Lean.Syntax → MetaM Expr
+def elabLFVar [MkLExprParams T] : Lean.Syntax → MetaM Expr
   | `(lfvar| $i:lident) => do
     let none ← mkNone (mkConst ``LTy)
     let metadata ← mkAppM ``Unit.unit #[]
-    let baseParams := mkApp2 (mkConst ``LExprParams.mk) (mkConst ``Unit) (MkLExprParams.toExpr IDMeta)
+    let baseParams := MkLExprParams.toExpr T
     let tParams := mkApp2 (mkConst ``LExprParamsT.mk) baseParams (mkConst ``LTy)
-    return mkAppN (.const ``LExpr.fvar []) #[tParams, metadata, ← MkLExprParams.elabIdent IDMeta i, none]
+    return mkAppN (.const ``LExpr.fvar []) #[tParams, metadata, ← MkLExprParams.elabIdent T i, none]
   | `(lfvar| ($i:lident : $ty:lty)) => do
     let lty ← Lambda.LTy.Syntax.elabLTy ty
     let lty ← mkSome (mkConst ``LTy) lty
     let metadata ← mkAppM ``Unit.unit #[]
-    let baseParams := mkApp2 (mkConst ``LExprParams.mk) (mkConst ``Unit) (MkLExprParams.toExpr IDMeta)
+    let baseParams := MkLExprParams.toExpr T
     let tParams := mkApp2 (mkConst ``LExprParamsT.mk) baseParams (mkConst ``LTy)
-    return mkAppN (.const ``LExpr.fvar []) #[tParams, metadata, ← MkLExprParams.elabIdent IDMeta i, lty]
+    return mkAppN (.const ``LExpr.fvar []) #[tParams, metadata, ← MkLExprParams.elabIdent T i, lty]
   | _ => throwUnsupportedSyntax
 scoped syntax lfvar : lexpr
 
@@ -1146,108 +1153,108 @@ open LTy.Syntax in
 It's the user's responsibility to ensure correct usage of type variables (i.e., they're
 unique).
 -/
-partial def elabLExpr (IDMeta : Type) [MkLExprParams IDMeta] : Lean.Syntax → MetaM Expr
-  | `(lexpr| $c:lconst) => elabLConst IDMeta c
-  | `(lexpr| $o:lop) => elabLOp IDMeta o
-  | `(lexpr| $b:lbvar) => elabLBVar IDMeta b
-  | `(lexpr| $f:lfvar) => elabLFVar IDMeta f
+partial def elabLExpr [MkLExprParams T] : Lean.Syntax → MetaM Expr
+  | `(lexpr| $c:lconst) => elabLConst (T:=T) c
+  | `(lexpr| $o:lop) => elabLOp (T:=T) o
+  | `(lexpr| $b:lbvar) => elabLBVar (T:=T) b
+  | `(lexpr| $f:lfvar) => elabLFVar (T:=T) f
   | `(lexpr| λ $e:lexpr) => do
-     let e' ← elabLExpr IDMeta e
+     let e' ← elabLExpr (T:=T) e
      let metadata ← mkAppM ``Unit.unit #[]
-     let baseParams := mkApp2 (mkConst ``LExprParams.mk) (mkConst ``Unit) (MkLExprParams.toExpr IDMeta)
+     let baseParams := MkLExprParams.toExpr T
      let tParams := mkApp2 (mkConst ``LExprParamsT.mk) baseParams (mkConst ``LTy)
      return mkAppN (.const ``LExpr.absUntyped []) #[tParams, metadata, e']
   | `(lexpr| λ ($mty:lty): $e:lexpr) => do
      let lty ← Lambda.LTy.Syntax.elabLTy mty
      let lty ← mkSome (mkConst ``LTy) lty
-     let e' ← elabLExpr IDMeta e
+     let e' ← elabLExpr (T:=T) e
      let metadata ← mkAppM ``Unit.unit #[]
-     let baseParams := mkApp2 (mkConst ``LExprParams.mk) (mkConst ``Unit) (MkLExprParams.toExpr IDMeta)
+     let baseParams := MkLExprParams.toExpr T
      let tParams := mkApp2 (mkConst ``LExprParamsT.mk) baseParams (mkConst ``LTy)
      return mkAppN (.const ``LExpr.abs []) #[tParams, metadata, lty, e']
   | `(lexpr| ∀ $e:lexpr) => do
-     let e' ← elabLExpr IDMeta e
+     let e' ← elabLExpr (T:=T) e
      let metadata ← mkAppM ``Unit.unit #[]
-     let baseParams := mkApp2 (mkConst ``LExprParams.mk) (mkConst ``Unit) (MkLExprParams.toExpr IDMeta)
+     let baseParams := MkLExprParams.toExpr T
      let tParams := mkApp2 (mkConst ``LExprParamsT.mk) baseParams (mkConst ``LTy)
      return mkAppN (.const ``LExpr.allUntyped []) #[tParams, metadata, e']
   | `(lexpr| ∀{$tr}$e:lexpr) => do
-     let e' ← elabLExpr IDMeta e
-     let tr' ← elabLExpr IDMeta tr
+     let e' ← elabLExpr (T:=T) e
+     let tr' ← elabLExpr (T:=T) tr
      let metadata ← mkAppM ``Unit.unit #[]
-     let baseParams := mkApp2 (mkConst ``LExprParams.mk) (mkConst ``Unit) (MkLExprParams.toExpr IDMeta)
+     let baseParams := MkLExprParams.toExpr T
      let tParams := mkApp2 (mkConst ``LExprParamsT.mk) baseParams (mkConst ``LTy)
      return mkAppN (.const ``LExpr.allUntypedTr []) #[tParams, metadata, tr', e']
   | `(lexpr| ∀ ($mty:lty): $e:lexpr) => do
      let lty ← Lambda.LTy.Syntax.elabLTy mty
      let lty ← mkSome (mkConst ``LTy) lty
-     let e' ← elabLExpr IDMeta e
+     let e' ← elabLExpr (T:=T) e
      let metadata ← mkAppM ``Unit.unit #[]
-     let baseParams := mkApp2 (mkConst ``LExprParams.mk) (mkConst ``Unit) (MkLExprParams.toExpr IDMeta)
+     let baseParams := MkLExprParams.toExpr T
      let tParams := mkApp2 (mkConst ``LExprParamsT.mk) baseParams (mkConst ``LTy)
      return mkAppN (.const ``LExpr.all []) #[tParams, metadata, lty, e']
   | `(lexpr| ∀ ($mty:lty): {$tr}$e:lexpr) => do
      let lty ← Lambda.LTy.Syntax.elabLTy mty
      let lty ← mkSome (mkConst ``LTy) lty
-     let e' ← elabLExpr IDMeta e
-     let tr' ← elabLExpr IDMeta tr
+     let e' ← elabLExpr (T:=T) e
+     let tr' ← elabLExpr (T:=T) tr
      let metadata ← mkAppM ``Unit.unit #[]
-     let baseParams := mkApp2 (mkConst ``LExprParams.mk) (mkConst ``Unit) (MkLExprParams.toExpr IDMeta)
+     let baseParams := MkLExprParams.toExpr T
      let tParams := mkApp2 (mkConst ``LExprParamsT.mk) baseParams (mkConst ``LTy)
      return mkAppN (.const ``LExpr.allTr []) #[tParams, metadata, lty, tr', e']
   | `(lexpr| ∃ ($mty:lty): $e:lexpr) => do
      let lty ← Lambda.LTy.Syntax.elabLTy mty
      let lty ← mkSome (mkConst ``LTy) lty
-     let e' ← elabLExpr IDMeta e
+     let e' ← elabLExpr (T:=T) e
      let metadata ← mkAppM ``Unit.unit #[]
-     let baseParams := mkApp2 (mkConst ``LExprParams.mk) (mkConst ``Unit) (MkLExprParams.toExpr IDMeta)
+     let baseParams := MkLExprParams.toExpr T
      let tParams := mkApp2 (mkConst ``LExprParamsT.mk) baseParams (mkConst ``LTy)
      return mkAppN (.const ``LExpr.exist []) #[tParams, metadata, lty, e']
   | `(lexpr| ∃ ($mty:lty): {$tr}$e:lexpr) => do
      let lty ← Lambda.LTy.Syntax.elabLTy mty
      let lty ← mkSome (mkConst ``LTy) lty
-     let e' ← elabLExpr IDMeta e
-     let tr' ← elabLExpr IDMeta tr
+     let e' ← elabLExpr (T:=T) e
+     let tr' ← elabLExpr (T:=T) tr
      let metadata ← mkAppM ``Unit.unit #[]
-     let baseParams := mkApp2 (mkConst ``LExprParams.mk) (mkConst ``Unit) (MkLExprParams.toExpr IDMeta)
+     let baseParams := MkLExprParams.toExpr T
      let tParams := mkApp2 (mkConst ``LExprParamsT.mk) baseParams (mkConst ``LTy)
      return mkAppN (.const ``LExpr.existTr []) #[tParams, metadata, lty, tr', e']
   | `(lexpr| ∃ $e:lexpr) => do
-     let e' ← elabLExpr IDMeta e
+     let e' ← elabLExpr (T:=T) e
      let metadata ← mkAppM ``Unit.unit #[]
-     let baseParams := mkApp2 (mkConst ``LExprParams.mk) (mkConst ``Unit) (MkLExprParams.toExpr IDMeta)
+     let baseParams := MkLExprParams.toExpr T
      let tParams := mkApp2 (mkConst ``LExprParamsT.mk) baseParams (mkConst ``LTy)
      return mkAppN (.const ``LExpr.existUntyped []) #[tParams, metadata, e']
   | `(lexpr| ∃ {$tr} $e:lexpr) => do
-     let e' ← elabLExpr IDMeta e
-     let tr' ← elabLExpr IDMeta tr
+     let e' ← elabLExpr (T:=T) e
+     let tr' ← elabLExpr (T:=T) tr
      let metadata ← mkAppM ``Unit.unit #[]
-     let baseParams := mkApp2 (mkConst ``LExprParams.mk) (mkConst ``Unit) (MkLExprParams.toExpr IDMeta)
+     let baseParams := MkLExprParams.toExpr T
      let tParams := mkApp2 (mkConst ``LExprParamsT.mk) baseParams (mkConst ``LTy)
      return mkAppN (.const ``LExpr.existUntypedTr []) #[tParams, metadata, tr', e']
   | `(lexpr| ($e1:lexpr $e2:lexpr)) => do
-     let e1' ← elabLExpr IDMeta e1
-     let e2' ← elabLExpr IDMeta e2
+     let e1' ← elabLExpr (T:=T) e1
+     let e2' ← elabLExpr (T:=T) e2
      let metadata ← mkAppM ``Unit.unit #[]
-     let baseParams := mkApp2 (mkConst ``LExprParams.mk) (mkConst ``Unit) (MkLExprParams.toExpr IDMeta)
+     let baseParams := MkLExprParams.toExpr T
      let tParams := mkApp2 (mkConst ``LExprParamsT.mk) baseParams (mkConst ``LTy)
      return mkAppN (.const ``LExpr.app []) #[tParams, metadata, e1', e2']
   | `(lexpr| $e1:lexpr == $e2:lexpr) => do
-     let e1' ← elabLExpr IDMeta e1
-     let e2' ← elabLExpr IDMeta e2
+     let e1' ← elabLExpr (T:=T) e1
+     let e2' ← elabLExpr (T:=T) e2
      let metadata ← mkAppM ``Unit.unit #[]
-     let baseParams := mkApp2 (mkConst ``LExprParams.mk) (mkConst ``Unit) (MkLExprParams.toExpr IDMeta)
+     let baseParams := MkLExprParams.toExpr T
      let tParams := mkApp2 (mkConst ``LExprParamsT.mk) baseParams (mkConst ``LTy)
      return mkAppN (.const ``LExpr.eq []) #[tParams, metadata, e1', e2']
   | `(lexpr| if $e1:lexpr then $e2:lexpr else $e3:lexpr) => do
-     let e1' ← elabLExpr IDMeta e1
-     let e2' ← elabLExpr IDMeta e2
-     let e3' ← elabLExpr IDMeta e3
+     let e1' ← elabLExpr (T:=T) e1
+     let e2' ← elabLExpr (T:=T) e2
+     let e3' ← elabLExpr (T:=T) e3
      let metadata ← mkAppM ``Unit.unit #[]
-     let baseParams := mkApp2 (mkConst ``LExprParams.mk) (mkConst ``Unit) (MkLExprParams.toExpr IDMeta)
+     let baseParams := MkLExprParams.toExpr T
      let tParams := mkApp2 (mkConst ``LExprParamsT.mk) baseParams (mkConst ``LTy)
      return mkAppN (.const ``LExpr.ite []) #[tParams, metadata, e1', e2', e3']
-  | `(lexpr| ($e:lexpr)) => elabLExpr IDMeta e
+  | `(lexpr| ($e:lexpr)) => elabLExpr (T:=T) e
   | _ => throwUnsupportedSyntax
 
 scoped syntax ident : lident
@@ -1258,13 +1265,18 @@ def elabStrIdent : Lean.Syntax → MetaM Expr
     return mkAppN (.const `Lambda.Identifier.mk []) #[.const ``Unit [], mkStrLit s.toString, .const ``Unit.unit []]
   | _ => throwUnsupportedSyntax
 
-instance : MkLExprParams Unit where
+instance : MkLExprParams ⟨Unit, Unit⟩ where
   elabIdent := elabStrIdent
-  toExpr := .const ``Unit []
+  toExpr := mkApp2 (mkConst ``LExprParams.mk) (mkConst ``Unit) (mkConst ``Unit)
 
-elab "es[" e:lexpr "]" : term => elabLExpr (IDMeta:=Unit) e
+elab "es[" e:lexpr "]" : term => elabLExpr (T:=⟨Unit, Unit⟩) e
 
 open LTy.Syntax
+/--
+info: const () (LConst.intConst (Int.ofNat 5)) : LExpr { base := { Metadata := Unit, IDMeta := Unit }, TypeType := LTy }
+-/
+#guard_msgs in
+#check es[#5]
 
 /--
 info: app () (absUntyped () (bvar () 0))
