Strata/Languages/Boogie/CmdType.lean
@@ -24,23 +24,13 @@ def isBoolType (ty : LTy) : Bool :=
   | .forAll [] LMonoTy.bool => true
   | _ => false
 
-<<<<<<< HEAD
-def lookup (Env : (TEnv BoogieLParams)) (x : BoogieIdent) : Option LTy :=
+def lookup (Env : TEnv Visibility) (x : BoogieIdent) : Option LTy :=
   Env.context.types.find? x
 
-def update (Env : TEnv BoogieLParams) (x : BoogieIdent) (ty : LTy) : TEnv BoogieLParams :=
-  Env.insertInContext x ty
+def update (Env : TEnv Visibility) (x : BoogieIdent) (ty : LTy) : TEnv Visibility :=
+  Env.insertInContext (T := BoogieLParams) x ty
 
 def freeVars (e : (LExpr BoogieLParams.mono)) : List BoogieIdent :=
-=======
-def lookup (T : (TEnv Visibility)) (x : BoogieIdent) : Option LTy :=
-  T.context.types.find? x
-
-def update (T : TEnv Visibility) (x : BoogieIdent) (ty : LTy) : TEnv Visibility :=
-  T.insertInContext x ty
-
-def freeVars (e : (LExpr LMonoTy Visibility)) : List BoogieIdent :=
->>>>>>> origin/main
   (LExpr.freeVars e).map (fun (i, _) => i)
 
 /--
@@ -48,25 +38,14 @@ Preprocess a user-facing type in Boogie amounts to converting a poly-type (i.e.,
 `LTy`) to a mono-type (i.e., `LMonoTy`) via instantiation. We still return an
 `LTy`, with no bound variables.
 -/
-<<<<<<< HEAD
-def preprocess (Env : TEnv BoogieLParams) (ty : LTy) : Except Format (LTy × TEnv BoogieLParams) := do
-  let (mty, Env) ← ty.instantiateWithCheck Env
+def preprocess (C: LContext BoogieLParams) (Env : TEnv Visibility) (ty : LTy) : Except Format (LTy × TEnv Visibility) := do
+  let (mty, Env) ← ty.instantiateWithCheck C Env
   return (.forAll [] mty, Env)
 
-def postprocess (Env: TEnv BoogieLParams) (ty : LTy) : Except Format (LTy × TEnv BoogieLParams) := do
+def postprocess (_: LContext BoogieLParams) (Env: TEnv Visibility) (ty : LTy) : Except Format (LTy × TEnv Visibility) := do
   if h: ty.isMonoType then
-    let ty := LMonoTy.subst Env.state.substInfo.subst (ty.toMonoType h)
+    let ty := LMonoTy.subst Env.stateSubstInfo.subst (ty.toMonoType h)
     .ok (.forAll [] ty, Env)
-=======
-def preprocess (C: LContext Visibility) (T : TEnv Visibility) (ty : LTy) : Except Format (LTy × TEnv Visibility) := do
-  let (mty, T) ← ty.instantiateWithCheck C T
-  return (.forAll [] mty, T)
-
-def postprocess (_: LContext Visibility) (T : TEnv Visibility) (ty : LTy) : Except Format (LTy × TEnv Visibility) := do
-  if h: ty.isMonoType then
-    let ty := LMonoTy.subst T.stateSubstInfo.subst (ty.toMonoType h)
-    .ok (.forAll [] ty, T)
->>>>>>> origin/main
   else
     .error f!"[postprocess] Expected mono-type; instead got {ty}"
 
@@ -74,13 +53,8 @@ def postprocess (_: LContext Visibility) (T : TEnv Visibility) (ty : LTy) : Exce
 The inferred type of `e` will be an `LMonoTy`, but we return an `LTy` with no
 bound variables.
 -/
-<<<<<<< HEAD
-def inferType (Env: TEnv BoogieLParams) (c : Cmd Expression) (e : (LExpr BoogieLParams.mono)) :
-    Except Format ((LExpr BoogieLParams.mono) × LTy × TEnv BoogieLParams) := do
-=======
-def inferType (C: LContext Visibility) (T : TEnv Visibility) (c : Cmd Expression) (e : (LExpr LMonoTy Visibility)) :
-    Except Format ((LExpr LMonoTy Visibility) × LTy × TEnv Visibility) := do
->>>>>>> origin/main
+def inferType (C: LContext BoogieLParams) (Env: TEnv Visibility) (c : Cmd Expression) (e : LExpr BoogieLParams.mono) :
+    Except Format ((LExpr BoogieLParams.mono) × LTy × TEnv Visibility) := do
   -- We only allow free variables to appear in `init` statements. Any other
   -- occurrence leads to an error.
   let T ← match c with
@@ -91,11 +65,7 @@ def inferType (C: LContext Visibility) (T : TEnv Visibility) (c : Cmd Expression
       let _ ← Env.freeVarCheck e f!"[{c}]"
       .ok Env
   let e := OldExpressions.normalizeOldExpr e
-<<<<<<< HEAD
-  let (ea, T) ← LExpr.fromLExpr T e
-=======
-  let (ea, T) ← LExprT.fromLExpr C T e
->>>>>>> origin/main
+  let (ea, T) ← LExpr.fromLExpr C T e
   let ety := ea.toLMonoTy
   return (ea.unresolved, (.forAll [] ety), T)
 
@@ -118,27 +88,15 @@ def canonicalizeConstraints (constraints : List (LTy × LTy)) : Except Format Co
                 type constraints, but found the following instead:\n\
                 t1: {t1}\nt2: {t2}\n"
 
-<<<<<<< HEAD
-def unifyTypes (Env: TEnv BoogieLParams) (constraints : List (LTy × LTy)) : Except Format (TEnv BoogieLParams) := do
+def unifyTypes (Env: TEnv Visibility) (constraints : List (LTy × LTy)) : Except Format (TEnv Visibility) := do
   let constraints ← canonicalizeConstraints constraints
-  let S ← Constraints.unify constraints Env.state.substInfo
+  let S ← Constraints.unify constraints Env.stateSubstInfo
   let Env := Env.updateSubst S
   return Env
 
 ---------------------------------------------------------------------
 
-instance : Imperative.TypeContext Expression (TEnv BoogieLParams) where
-=======
-def unifyTypes (T : TEnv Visibility) (constraints : List (LTy × LTy)) : Except Format (TEnv Visibility) := do
-  let constraints ← canonicalizeConstraints constraints
-  let S ← Constraints.unify constraints T.stateSubstInfo
-  let T := T.updateSubst S
-  return T
-
----------------------------------------------------------------------
-
-instance : Imperative.TypeContext Expression (LContext Visibility) (TEnv Visibility) where
->>>>>>> origin/main
+instance : Imperative.TypeContext Expression (LContext BoogieLParams) (TEnv Visibility) where
   isBoolType  := CmdType.isBoolType
   freeVars    := CmdType.freeVars
   preprocess  := CmdType.preprocess
