Strata/Languages/Boogie/Examples/DDMAxiomsExtraction.lean
@@ -36,11 +36,7 @@ def extractAxiomsDecl (prg: Boogie.Program) : (List Boogie.Decl) :=
 /--
   Extract the body LExpr from the axiom declaration
 -/
-<<<<<<< HEAD
 def extractExpr (axDecl: Boogie.Decl): Boogie.Expression.Expr :=
-=======
-def extractExpr (axDecl: Boogie.Decl): (Lambda.LExpr Lambda.LMonoTy Boogie.Visibility) :=
->>>>>>> origin/main
   match axDecl with
     | .ax a _ => a.e
     | _ => panic "Can be called only on axiom declaration"
@@ -65,10 +61,9 @@ def transformSimpleTypeToFreeVariable (ty: Lambda.LMonoTy) (to_replace: List Str
   Transform all occurences of types of the form LMonoTy.tcons name [] into ftvar name, if name is in to_replace
   in the given expression
 -/
-<<<<<<< HEAD
 def replaceTypesByFTV (expr: Boogie.Expression.Expr) (to_replace: List String): Boogie.Expression.Expr :=
   match expr with
-    | .const m c oty => .const m c (oty.map (fun t => transformSimpleTypeToFreeVariable t to_replace))
+    | .const m c => .const m c
     | .op m o oty => .op m o (oty.map (fun t => transformSimpleTypeToFreeVariable t to_replace))
     | .fvar m name oty => .fvar m name (oty.map (fun t => transformSimpleTypeToFreeVariable t to_replace))
     | .bvar m i => .bvar m i
@@ -77,30 +72,12 @@ def replaceTypesByFTV (expr: Boogie.Expression.Expr) (to_replace: List String): 
     | .app m fn e => .app m (replaceTypesByFTV fn to_replace) (replaceTypesByFTV e to_replace)
     | .ite m c t e => .ite m (replaceTypesByFTV c to_replace) (replaceTypesByFTV t to_replace) (replaceTypesByFTV e to_replace)
     | .eq m e1 e2 => .eq m (replaceTypesByFTV e1 to_replace) (replaceTypesByFTV e2 to_replace)
-=======
-def replaceTypesByFTV (expr: Lambda.LExpr Lambda.LMonoTy Boogie.Visibility) (to_replace: List String): Lambda.LExpr Lambda.LMonoTy Boogie.Visibility :=
-  match expr with
-    | .const c => .const c
-    | .op o oty => .op o (oty.map (fun t => transformSimpleTypeToFreeVariable t to_replace))
-    | .fvar name oty => .fvar name (oty.map (fun t => transformSimpleTypeToFreeVariable t to_replace))
-    | .mdata info e => .mdata info (replaceTypesByFTV e to_replace)
-    | .abs oty e => .abs (oty.map (fun t => transformSimpleTypeToFreeVariable t to_replace)) (replaceTypesByFTV e to_replace)
-    | .quant k oty tr e => .quant k (oty.map (fun t => transformSimpleTypeToFreeVariable t to_replace)) (replaceTypesByFTV tr to_replace) (replaceTypesByFTV e to_replace)
-    | .app fn e => .app (replaceTypesByFTV fn to_replace) (replaceTypesByFTV e to_replace)
-    | .ite c t e => .ite (replaceTypesByFTV c to_replace) (replaceTypesByFTV t to_replace) (replaceTypesByFTV e to_replace)
-    | .eq e1 e2 => .eq (replaceTypesByFTV e1 to_replace) (replaceTypesByFTV e2 to_replace)
-    | _ => expr
->>>>>>> origin/main
 
 /--
   Extract all axioms from the given environment by first translating it into a Boogie Program.
   It then extracts LExpr body from the axioms, and replace all occurences of the typeArgs by a ftvar with the same name
 -/
-<<<<<<< HEAD
 def extractAxiomsWithFreeTypeVars (pgm: Program) (typeArgs: List String): (List Boogie.Expression.Expr) :=
-=======
-def extractAxiomsWithFreeTypeVars (pgm: Program) (typeArgs: List String): (List (Lambda.LExpr Lambda.LMonoTy Boogie.Visibility)) :=
->>>>>>> origin/main
   let prg: Boogie.Program := (TransM.run (translateProgram pgm)).fst
   let axiomsDecls := extractAxiomsDecl prg
   let axioms := axiomsDecls.map extractExpr
@@ -418,21 +395,22 @@ info: #[{ ann := { start := { byteIdx := 295 }, stop := { byteIdx := 302 } },
 #eval examplePgm.commands
 
 /--
-<<<<<<< HEAD
 info: [LExpr.quant () QuantifierKind.all (some Lambda.LMonoTy.tcons
    "Map"
    [Lambda.LMonoTy.ftvar "k",
     Lambda.LMonoTy.ftvar
       "v"]) (LExpr.bvar () 0) (LExpr.quant () QuantifierKind.all (some Lambda.LMonoTy.ftvar
    "k") (LExpr.bvar () 0) (LExpr.quant () QuantifierKind.all (some Lambda.LMonoTy.ftvar
-   "v") (LExpr.bvar () 0) (LExpr.eq () (LExpr.app () (LExpr.app () (LExpr.op () u:select (some Lambda.LMonoTy.tcons
+   "v") (LExpr.bvar () 0) (LExpr.eq () (LExpr.app () (LExpr.app () (LExpr.op () { name := "select",
+   metadata := Boogie.Visibility.unres } (some Lambda.LMonoTy.tcons
    "arrow"
    [Lambda.LMonoTy.tcons "Map" [Lambda.LMonoTy.ftvar "k", Lambda.LMonoTy.ftvar "v"],
     Lambda.LMonoTy.tcons
       "arrow"
       [Lambda.LMonoTy.ftvar "k",
        Lambda.LMonoTy.ftvar
-         "v"]])) (LExpr.app () (LExpr.app () (LExpr.app () (LExpr.op () u:update (some Lambda.LMonoTy.tcons
+         "v"]])) (LExpr.app () (LExpr.app () (LExpr.app () (LExpr.op () { name := "update",
+   metadata := Boogie.Visibility.unres } (some Lambda.LMonoTy.tcons
    "arrow"
    [Lambda.LMonoTy.tcons "Map" [Lambda.LMonoTy.ftvar "k", Lambda.LMonoTy.ftvar "v"],
     Lambda.LMonoTy.tcons
@@ -453,14 +431,16 @@ info: [LExpr.quant () QuantifierKind.all (some Lambda.LMonoTy.tcons
       "v"]) (LExpr.bvar () 0) (LExpr.quant () QuantifierKind.all (some Lambda.LMonoTy.ftvar
    "k") (LExpr.bvar () 0) (LExpr.quant () QuantifierKind.all (some Lambda.LMonoTy.ftvar
    "k") (LExpr.bvar () 0) (LExpr.quant () QuantifierKind.all (some Lambda.LMonoTy.ftvar
-   "v") (LExpr.bvar () 0) (LExpr.eq () (LExpr.app () (LExpr.app () (LExpr.op () u:select (some Lambda.LMonoTy.tcons
+   "v") (LExpr.bvar () 0) (LExpr.eq () (LExpr.app () (LExpr.app () (LExpr.op () { name := "select",
+   metadata := Boogie.Visibility.unres } (some Lambda.LMonoTy.tcons
    "arrow"
    [Lambda.LMonoTy.tcons "Map" [Lambda.LMonoTy.ftvar "k", Lambda.LMonoTy.ftvar "v"],
     Lambda.LMonoTy.tcons
       "arrow"
       [Lambda.LMonoTy.ftvar "k",
        Lambda.LMonoTy.ftvar
-         "v"]])) (LExpr.app () (LExpr.app () (LExpr.app () (LExpr.op () u:update (some Lambda.LMonoTy.tcons
+         "v"]])) (LExpr.app () (LExpr.app () (LExpr.app () (LExpr.op () { name := "update",
+   metadata := Boogie.Visibility.unres } (some Lambda.LMonoTy.tcons
    "arrow"
    [Lambda.LMonoTy.tcons "Map" [Lambda.LMonoTy.ftvar "k", Lambda.LMonoTy.ftvar "v"],
     Lambda.LMonoTy.tcons
@@ -473,109 +453,13 @@ info: [LExpr.quant () QuantifierKind.all (some Lambda.LMonoTy.tcons
             "Map"
             [Lambda.LMonoTy.ftvar "k",
              Lambda.LMonoTy.ftvar
-               "v"]]]])) (LExpr.bvar () 3)) (LExpr.bvar () 1)) (LExpr.bvar () 0))) (LExpr.bvar () 2)) (LExpr.app () (LExpr.app () (LExpr.op () u:select (some Lambda.LMonoTy.tcons
+               "v"]]]])) (LExpr.bvar () 3)) (LExpr.bvar () 1)) (LExpr.bvar () 0))) (LExpr.bvar () 2)) (LExpr.app () (LExpr.app () (LExpr.op () { name := "select",
+   metadata := Boogie.Visibility.unres } (some Lambda.LMonoTy.tcons
    "arrow"
    [Lambda.LMonoTy.tcons "Map" [Lambda.LMonoTy.ftvar "k", Lambda.LMonoTy.ftvar "v"],
     Lambda.LMonoTy.tcons
       "arrow"
       [Lambda.LMonoTy.ftvar "k", Lambda.LMonoTy.ftvar "v"]])) (LExpr.bvar () 3)) (LExpr.bvar () 2))))))]
-=======
-info: [Lambda.LExpr.quant
-   (Lambda.QuantifierKind.all)
-   (some (Lambda.LMonoTy.tcons "Map" [Lambda.LMonoTy.ftvar "k", Lambda.LMonoTy.ftvar "v"]))
-   (Lambda.LExpr.bvar 0)
-   (Lambda.LExpr.quant
-     (Lambda.QuantifierKind.all)
-     (some (Lambda.LMonoTy.ftvar "k"))
-     (Lambda.LExpr.bvar 0)
-     (Lambda.LExpr.quant
-       (Lambda.QuantifierKind.all)
-       (some (Lambda.LMonoTy.ftvar "v"))
-       (Lambda.LExpr.bvar 0)
-       (Lambda.LExpr.eq
-         (Lambda.LExpr.app
-           (Lambda.LExpr.app
-             (Lambda.LExpr.op
-               { name := "select", metadata := Boogie.Visibility.unres }
-               (some (Lambda.LMonoTy.tcons
-                  "arrow"
-                  [Lambda.LMonoTy.tcons "Map" [Lambda.LMonoTy.ftvar "k", Lambda.LMonoTy.ftvar "v"],
-                   Lambda.LMonoTy.tcons "arrow" [Lambda.LMonoTy.ftvar "k", Lambda.LMonoTy.ftvar "v"]])))
-             (Lambda.LExpr.app
-               (Lambda.LExpr.app
-                 (Lambda.LExpr.app
-                   (Lambda.LExpr.op
-                     { name := "update", metadata := Boogie.Visibility.unres }
-                     (some (Lambda.LMonoTy.tcons
-                        "arrow"
-                        [Lambda.LMonoTy.tcons "Map" [Lambda.LMonoTy.ftvar "k", Lambda.LMonoTy.ftvar "v"],
-                         Lambda.LMonoTy.tcons
-                           "arrow"
-                           [Lambda.LMonoTy.ftvar "k",
-                            Lambda.LMonoTy.tcons
-                              "arrow"
-                              [Lambda.LMonoTy.ftvar "v",
-                               Lambda.LMonoTy.tcons "Map" [Lambda.LMonoTy.ftvar "k", Lambda.LMonoTy.ftvar "v"]]]])))
-                   (Lambda.LExpr.bvar 2))
-                 (Lambda.LExpr.bvar 1))
-               (Lambda.LExpr.bvar 0)))
-           (Lambda.LExpr.bvar 1))
-         (Lambda.LExpr.bvar 0)))),
- Lambda.LExpr.quant
-   (Lambda.QuantifierKind.all)
-   (some (Lambda.LMonoTy.tcons "Map" [Lambda.LMonoTy.ftvar "k", Lambda.LMonoTy.ftvar "v"]))
-   (Lambda.LExpr.bvar 0)
-   (Lambda.LExpr.quant
-     (Lambda.QuantifierKind.all)
-     (some (Lambda.LMonoTy.ftvar "k"))
-     (Lambda.LExpr.bvar 0)
-     (Lambda.LExpr.quant
-       (Lambda.QuantifierKind.all)
-       (some (Lambda.LMonoTy.ftvar "k"))
-       (Lambda.LExpr.bvar 0)
-       (Lambda.LExpr.quant
-         (Lambda.QuantifierKind.all)
-         (some (Lambda.LMonoTy.ftvar "v"))
-         (Lambda.LExpr.bvar 0)
-         (Lambda.LExpr.eq
-           (Lambda.LExpr.app
-             (Lambda.LExpr.app
-               (Lambda.LExpr.op
-                 { name := "select", metadata := Boogie.Visibility.unres }
-                 (some (Lambda.LMonoTy.tcons
-                    "arrow"
-                    [Lambda.LMonoTy.tcons "Map" [Lambda.LMonoTy.ftvar "k", Lambda.LMonoTy.ftvar "v"],
-                     Lambda.LMonoTy.tcons "arrow" [Lambda.LMonoTy.ftvar "k", Lambda.LMonoTy.ftvar "v"]])))
-               (Lambda.LExpr.app
-                 (Lambda.LExpr.app
-                   (Lambda.LExpr.app
-                     (Lambda.LExpr.op
-                       { name := "update", metadata := Boogie.Visibility.unres }
-                       (some (Lambda.LMonoTy.tcons
-                          "arrow"
-                          [Lambda.LMonoTy.tcons "Map" [Lambda.LMonoTy.ftvar "k", Lambda.LMonoTy.ftvar "v"],
-                           Lambda.LMonoTy.tcons
-                             "arrow"
-                             [Lambda.LMonoTy.ftvar "k",
-                              Lambda.LMonoTy.tcons
-                                "arrow"
-                                [Lambda.LMonoTy.ftvar "v",
-                                 Lambda.LMonoTy.tcons "Map" [Lambda.LMonoTy.ftvar "k", Lambda.LMonoTy.ftvar "v"]]]])))
-                     (Lambda.LExpr.bvar 3))
-                   (Lambda.LExpr.bvar 1))
-                 (Lambda.LExpr.bvar 0)))
-             (Lambda.LExpr.bvar 2))
-           (Lambda.LExpr.app
-             (Lambda.LExpr.app
-               (Lambda.LExpr.op
-                 { name := "select", metadata := Boogie.Visibility.unres }
-                 (some (Lambda.LMonoTy.tcons
-                    "arrow"
-                    [Lambda.LMonoTy.tcons "Map" [Lambda.LMonoTy.ftvar "k", Lambda.LMonoTy.ftvar "v"],
-                     Lambda.LMonoTy.tcons "arrow" [Lambda.LMonoTy.ftvar "k", Lambda.LMonoTy.ftvar "v"]])))
-               (Lambda.LExpr.bvar 3))
-             (Lambda.LExpr.bvar 2))))))]
->>>>>>> origin/main
 -/
 #guard_msgs in
 #eval
