Strata/Languages/Boogie/Function.lean
@@ -17,37 +17,24 @@ open Lambda
 
 /-! # Boogie Functions -/
 
-<<<<<<< HEAD
 abbrev Function := Lambda.LFunc BoogieLParams
 
 -- Type class instances to enable type class resolution for BoogieLParams.Identifier
-instance : DecidableEq BoogieLParams.Identifier :=
-  show DecidableEq BoogieIdent from inferInstance
+instance : DecidableEq BoogieLParams.IDMeta :=
+  show DecidableEq Visibility from inferInstance
 
-instance : ToFormat BoogieLParams.Identifier :=
-  show ToFormat BoogieIdent from inferInstance
-=======
-abbrev Function := Lambda.LFunc BoogieLParams
->>>>>>> origin/main
+instance : ToFormat BoogieLParams.IDMeta :=
+  show ToFormat Visibility from inferInstance
 
 open LTy.Syntax LExpr.SyntaxMono in
 /-- info: ok: ∀[a, b]. (arrow int (arrow a (arrow b (arrow a a)))) -/
 #guard_msgs in
-<<<<<<< HEAD
 #eval do let type ← LFunc.type (T:=BoogieLParams)
                      ({ name := BoogieIdent.unres "Foo",
                         typeArgs := ["a", "b"],
                         inputs := [(BoogieIdent.locl "w", mty[int]), (BoogieIdent.locl "x", mty[%a]), (BoogieIdent.locl "y", mty[%b]), (BoogieIdent.locl "z", mty[%a])],
                         output := mty[%a],
                         body := some (LExpr.fvar () (BoogieIdent.locl "x") none) } : Function)
-=======
-#eval do let type ← LFunc.type (IDMeta:=Visibility)
-                     ({ name := (BoogieIdent.unres "Foo"),
-                        typeArgs := ["a", "b"],
-                        inputs := [((BoogieIdent.locl "w"), mty[int]), ((BoogieIdent.locl "x"), mty[%a]), ((BoogieIdent.locl "y"), mty[%b]), ((BoogieIdent.locl "z"), mty[%a])],
-                        output := mty[%a],
-                        body := some (.fvar (BoogieIdent.locl "x") none) } : Function)
->>>>>>> origin/main
          return format type
 
 ---------------------------------------------------------------------
