Strata/Languages/Boogie/StatementType.lean
@@ -25,21 +25,12 @@ Type checker for Boogie commands.
 Note that this function needs the entire program to type-check `call`
 commands by looking up the corresponding procedure's information.
 -/
-<<<<<<< HEAD
-def typeCheckCmd (Env : TEnv BoogieLParams) (P : Program) (c : Command) :
-  Except Format (Command × TEnv BoogieLParams) := do
-  match c with
-  | .cmd c =>
-    let (c, Env) ← Imperative.Cmd.typeCheck Env c
-    .ok (.cmd c, Env)
-=======
-def typeCheckCmd (C: LContext Visibility) (T : (TEnv Visibility)) (P : Program) (c : Command) :
+def typeCheckCmd (C: LContext BoogieLParams) (Env : TEnv Visibility) (P : Program) (c : Command) :
   Except Format (Command × (TEnv Visibility)) := do
   match c with
   | .cmd c =>
-    let (c, T) ← Imperative.Cmd.typeCheck C T c
-    .ok (.cmd c, T)
->>>>>>> origin/main
+    let (c, Env) ← Imperative.Cmd.typeCheck C Env c
+    .ok (.cmd c, Env)
   | .call lhs pname args md =>
      match Program.Procedure.find? P pname with
      | none => .error f!"[{c}]: Procedure {pname} not found!"
@@ -55,146 +46,78 @@ def typeCheckCmd (C: LContext Visibility) (T : (TEnv Visibility)) (P : Program) 
        else do
          -- Get the types of lhs variables and unify with the procedures'
          -- return types.
-<<<<<<< HEAD
-         let lhsinsts ← Identifier.instantiateAndSubsts lhs Env
+         let lhsinsts ← Lambda.Identifier.instantiateAndSubsts lhs C Env
          match lhsinsts with
          | none => .error f!"Implementation error. \
                              Types of {lhs} should have been known."
          | some (lhs_tys, Env) =>
            let _ ← Env.freeVarChecks args
-           let (ret_sig, Env) ← LMonoTySignature.instantiate Env proc.header.typeArgs proc.header.outputs
-           let ret_mtys := LMonoTys.subst Env.state.substInfo.subst ret_sig.values
+           let (ret_sig, Env) ← LMonoTySignature.instantiate C Env proc.header.typeArgs proc.header.outputs
+           let ret_mtys := LMonoTys.subst Env.stateSubstInfo.subst ret_sig.values
            let ret_lhs_constraints := lhs_tys.zip ret_mtys
            -- Infer the types of the actuals and unify with the types of the
            -- procedure's formals.
-           let (argsa, Env) ← LExpr.fromLExprs Env args
+           let (argsa, Env) ← Lambda.LExpr.fromLExprs C Env args
            let args_tys := argsa.map LExpr.toLMonoTy
            let args' := argsa.map $ LExpr.unresolved
-           let (inp_sig, Env) ← LMonoTySignature.instantiate Env proc.header.typeArgs proc.header.inputs
-           let inp_mtys := LMonoTys.subst Env.state.substInfo.subst inp_sig.values
+           let (inp_sig, Env) ← LMonoTySignature.instantiate C Env proc.header.typeArgs proc.header.inputs
+           let inp_mtys := LMonoTys.subst Env.stateSubstInfo.subst inp_sig.values
            let lhs_inp_constraints := (args_tys.zip inp_mtys)
-           let S ← Constraints.unify (lhs_inp_constraints ++ ret_lhs_constraints) Env.state.substInfo
+           let S ← Constraints.unify (lhs_inp_constraints ++ ret_lhs_constraints) Env.stateSubstInfo
            let Env := Env.updateSubst S
-=======
-         let lhsinsts ← Lambda.Identifier.instantiateAndSubsts lhs C T
-         match lhsinsts with
-         | none => .error f!"Implementation error. \
-                             Types of {lhs} should have been known."
-         | some (lhs_tys, T) =>
-           let _ ← T.freeVarChecks args
-           let (ret_sig, T) ← LMonoTySignature.instantiate C T proc.header.typeArgs proc.header.outputs
-           let ret_mtys := LMonoTys.subst T.stateSubstInfo.subst ret_sig.values
-           let ret_lhs_constraints := lhs_tys.zip ret_mtys
-           -- Infer the types of the actuals and unify with the types of the
-           -- procedure's formals.
-           let (argsa, T) ← Lambda.LExprT.fromLExprs C T args
-           let args_tys := argsa.map LExprT.toLMonoTy
-           let args' := argsa.map $ LExprT.toLExpr
-           let (inp_sig, T) ← LMonoTySignature.instantiate C T proc.header.typeArgs proc.header.inputs
-           let inp_mtys := LMonoTys.subst T.stateSubstInfo.subst inp_sig.values
-           let lhs_inp_constraints := (args_tys.zip inp_mtys)
-           let S ← Constraints.unify (lhs_inp_constraints ++ ret_lhs_constraints) T.stateSubstInfo
-           let T := T.updateSubst S
->>>>>>> origin/main
            let s' := .call lhs pname args' md
            .ok (s', Env)
 
 
-<<<<<<< HEAD
-def typeCheckAux (Env : TEnv BoogieLParams) (P : Program) (op : Option Procedure) (ss : List Statement) :
-  Except Format (List Statement × TEnv BoogieLParams) :=
+def typeCheckAux (C: LContext BoogieLParams) (Env : TEnv Visibility) (P : Program) (op : Option Procedure) (ss : List Statement) :
+  Except Format (List Statement × TEnv Visibility) :=
   go Env ss []
 where
-  go (Env : TEnv BoogieLParams) (ss : List Statement) (acc : List Statement) :
-    Except Format (List Statement × TEnv BoogieLParams) :=
-=======
-def typeCheckAux (C: LContext Visibility) (T : (TEnv Visibility)) (P : Program) (op : Option Procedure) (ss : List Statement) :
-  Except Format (List Statement × (TEnv Visibility)) :=
-  go T ss []
-where
-  go (T : TEnv Visibility) (ss : List Statement) (acc : List Statement) :
-    Except Format (List Statement × (TEnv Visibility)) :=
->>>>>>> origin/main
+  go (Env : TEnv Visibility) (ss : List Statement) (acc : List Statement) :
+    Except Format (List Statement × TEnv Visibility) :=
     match ss with
     | [] => .ok (acc.reverse, Env)
     | s :: srest => do
       let (s', Env) ←
         match s with
         | .cmd cmd => do
-<<<<<<< HEAD
-          let (c', Env) ← typeCheckCmd Env P cmd
+          let (c', Env) ← typeCheckCmd C Env P cmd
           .ok (.cmd c', Env)
 
-        | .block label blk md => do
-          let T := Env.pushEmptyContext
-          let (ss', T) ← go T blk.ss []
-          let s' := .block label ⟨ss'⟩ md
-          .ok (s', T.popContext)
-
-        | .ite cond thenb elseb md => do
-          let _ ← Env.freeVarChecks [cond]
-          let (conda, T) ← LExpr.fromLExpr Env cond
-          let condty := conda.toLMonoTy
-          match condty with
-          | .tcons "bool" [] =>
-            let (tb, T) ← go T [(.block "$$_then" thenb #[])] []
-            let (eb, T) ← go T [(.block "$$_else" elseb #[])] []
-            let s' := .ite conda.unresolved ⟨tb⟩ ⟨eb⟩ md
-            .ok (s', T)
-          | _ => .error f!"[{s}]: If's condition {cond} is not of type `bool`!"
-
-        | .loop guard measure invariant body md => do
-          let _ ← Env.freeVarChecks [guard]
-          let (conda, T) ← LExpr.fromLExpr Env guard
-          let condty := conda.toLMonoTy
-          let (mt, T) ← match measure with
-          | .some m => do
-            let _ ← T.freeVarChecks [m]
-            let (ma, T) ← LExpr.fromLExpr T m
-=======
-          let (c', T) ← typeCheckCmd C T P cmd
-          .ok (.cmd c', T)
-
         | .block label ⟨ bss ⟩ md => do
-          let T := T.pushEmptyContext
-          let (ss', T) ← go T bss []
+          let Env := Env.pushEmptyContext
+          let (ss', Env) ← go Env bss []
           let s' := .block label ⟨ss'⟩ md
-          .ok (s', T.popContext)
+          .ok (s', Env.popContext)
 
         | .ite cond ⟨ tss ⟩ ⟨ ess ⟩ md => do
-          let _ ← T.freeVarCheck cond f!"[{s}]"
-          let (conda, T) ← LExprT.fromLExpr C T cond
+          let _ ← Env.freeVarCheck cond f!"[{s}]"
+          let (conda, Env) ← LExpr.fromLExpr C Env cond
           let condty := conda.toLMonoTy
           match condty with
           | .tcons "bool" [] =>
-            let (tb, T) ← go T [(.block "$$_then" ⟨ tss ⟩  #[])] []
-            let (eb, T) ← go T [(.block "$$_else" ⟨ ess ⟩  #[])] []
-            let s' := .ite conda.toLExpr ⟨tb⟩ ⟨eb⟩ md
-            .ok (s', T)
+            let (tb, Env) ← go Env [(.block "$$_then" ⟨ tss ⟩  #[])] []
+            let (eb, Env) ← go Env [(.block "$$_else" ⟨ ess ⟩  #[])] []
+            let s' := .ite conda.unresolved ⟨tb⟩ ⟨eb⟩ md
+            .ok (s', Env)
           | _ => .error f!"[{s}]: If's condition {cond} is not of type `bool`!"
 
         | .loop guard measure invariant ⟨ bss ⟩ md => do
-          let _ ← T.freeVarCheck guard f!"[{s}]"
-          let (conda, T) ← LExprT.fromLExpr C T guard
+          let _ ← Env.freeVarCheck guard f!"[{s}]"
+          let (conda, Env) ← LExpr.fromLExpr C Env guard
           let condty := conda.toLMonoTy
-          let (mt, T) ← match measure with
+          let (mt, Env) ← match measure with
           | .some m => do
-            let _ ← T.freeVarCheck m f!"[{s}]"
-            let (ma, T) ← LExprT.fromLExpr C T m
->>>>>>> origin/main
-            .ok (some ma, T)
-          | _ => .ok (none, T)
-          let (it, T) ← match invariant with
+            let _ ← Env.freeVarCheck m f!"[{s}]"
+            let (ma, Env) ← LExpr.fromLExpr C Env m
+            .ok (some ma, Env)
+          | _ => .ok (none, Env)
+          let (it, Env) ← match invariant with
           | .some i => do
-<<<<<<< HEAD
-            let _ ← T.freeVarChecks [i]
-            let (ia, T) ← LExpr.fromLExpr T i
-=======
-            let _ ← T.freeVarCheck i f!"[{s}]"
-            let (ia, T) ← LExprT.fromLExpr C T i
->>>>>>> origin/main
-            .ok (some ia, T)
-          | _ => .ok (none, T)
+            let _ ← Env.freeVarCheck i f!"[{s}]"
+            let (ia, Env) ← LExpr.fromLExpr C Env i
+            .ok (some ia, Env)
+          | _ => .ok (none, Env)
           let mty := mt.map LExpr.toLMonoTy
           let ity := it.map LExpr.toLMonoTy
           match (condty, mty, ity) with
@@ -202,14 +125,9 @@ where
           | (.tcons "bool" [], some (.tcons "int" []), none)
           | (.tcons "bool" [], none, some (.tcons "bool" []))
           | (.tcons "bool" [], some (.tcons "int" []), some (.tcons "bool" [])) =>
-<<<<<<< HEAD
-            let (tb, T) ← go T [(.block "$$_loop_body" body #[])] []
+            let (tb, Env) ← go Env [(.block "$$_loop_body" ⟨bss⟩ #[])] []
             let s' := .loop conda.unresolved (mt.map LExpr.unresolved) (it.map LExpr.unresolved) ⟨tb⟩ md
-=======
-            let (tb, T) ← go T [(.block "$$_loop_body" ⟨ bss ⟩ #[])] []
-            let s' := .loop conda.toLExpr (mt.map LExprT.toLExpr) (it.map LExprT.toLExpr) ⟨tb⟩ md
->>>>>>> origin/main
-            .ok (s', T)
+            .ok (s', Env)
           | _ =>
             match condty with
             | .tcons "bool" [] =>
@@ -264,21 +182,12 @@ Apply type substitution `S` to a statement.
 def Statement.subst (S : Subst) (s : Statement) : Statement :=
   match s with
   | .cmd cmd => .cmd (Command.subst S cmd)
-<<<<<<< HEAD
-  | .block label b md =>
-    .block label ⟨go S b.ss []⟩ md
-  | .ite cond thenb elseb md =>
-    .ite (LExpr.applySubst cond S) ⟨go S thenb.ss []⟩ ⟨go S elseb.ss []⟩ md
-  | .loop guard m i body md =>
-    .loop (LExpr.applySubst guard S) (substOptionExpr S m) (substOptionExpr S i) ⟨go S body.ss []⟩ md
-=======
   | .block label ⟨ bss ⟩ md =>
     .block label ⟨go S bss []⟩ md
   | .ite cond ⟨ tss ⟩ ⟨ ess ⟩ md =>
     .ite (cond.applySubst S) ⟨go S tss []⟩ ⟨go S ess []⟩ md
   | .loop guard m i ⟨ bss ⟩ md =>
     .loop (guard.applySubst S) (substOptionExpr S m) (substOptionExpr S i) ⟨go S bss []⟩ md
->>>>>>> origin/main
   | .goto _ _ => s
   where
     go S ss acc : List Statement :=
@@ -293,22 +202,13 @@ Note that this function needs the entire program to type-check statements to
 check whether `goto` targets exist (or .none for statements that don't occur
 inside a procedure).
 -/
-<<<<<<< HEAD
-def typeCheck (T : TEnv BoogieLParams) (P : Program) (op : Option Procedure) (ss : List Statement) :
-  Except Format (List Statement × TEnv BoogieLParams) := do
-  let (ss', T) ← typeCheckAux T P op ss
-  let context := TContext.subst T.context T.state.substInfo.subst
-  let T := { T with context := context }
-  let ss' := Statement.subst.go T.state.substInfo.subst ss' []
-=======
-def typeCheck (C: Expression.TyContext) (T : Expression.TyEnv) (P : Program) (op : Option Procedure) (ss : List Statement) :
+def typeCheck (C: Expression.TyContext) (Env : Expression.TyEnv) (P : Program) (op : Option Procedure) (ss : List Statement) :
   Except Format (List Statement × Expression.TyEnv) := do
-  let (ss', T) ← typeCheckAux C T P op ss
-  let context := TContext.subst T.context T.stateSubstInfo.subst
-  let T := T.updateContext context
-  let ss' := Statement.subst.go T.stateSubstInfo.subst ss' []
->>>>>>> origin/main
-  .ok (ss', T)
+  let (ss', Env) ← typeCheckAux C Env P op ss
+  let context := TContext.subst Env.context Env.stateSubstInfo.subst
+  let Env := Env.updateContext context
+  let ss' := Statement.subst.go Env.stateSubstInfo.subst ss' []
+  .ok (ss', Env)
 
 ---------------------------------------------------------------------
 end Statement
